<?xml version="1.0" encoding="UTF-8"?>
<rdf:RDF xmlns:rdf="http://www.w3.org/1999/02/22-rdf-syntax-ns#"
  xmlns:owl="http://www.w3.org/2002/07/owl#"
  xmlns:dcterms="http://purl.org/dc/terms/"
  xmlns:vann="http://purl.org/vocab/vann/"
  xmlns:foaf="http://xmlns.com/foaf/0.1/"
  xmlns:dc="http://purl.org/dc/elements/1.1/"
  xmlns:adms="http://www.w3.org/ns/adms#"
  xmlns:rdfs="http://www.w3.org/2000/01/rdf-schema#">

  <owl:Ontology rdf:about="http://vocab.deri.ie/ac">
    <rdf:type rdf:resource="http://www.w3.org/ns/adms#SemanticAsset"/>
    <dcterms:title>Action Category Meta-Model</dcterms:title>
    <dcterms:description>This is an rdf schema for defining an ActionCategory. It defines the concept ActionCategory as an rdfs:Class. It defines for this concept three properties: (1) ac:hasPart which is an rdf:Property (2) ac:hasOptionalPart which is an rdf:Property, both of them are used to create meronymy relations between ActionCategories and (3) ac:hasLevel which is an owl:DatatypeProperty that indicates the level of the current action category in the hierarchy built using the two previous properties.</dcterms:description>
    <dcterms:modified rdf:datatype="http://www.w3.org/2001/XMLSchema#date">2015-05-08</dcterms:modified>
    <vann:preferredNamespaceUri>http://vocab.deri.ie/ac#</vann:preferredNamespaceUri>
    <vann:preferredNamespacePrefix>ac</vann:preferredNamespacePrefix>
    <foaf:homepage rdf:resource="http://vocab.deri.ie/ac.html"/>
    <dcterms:created rdf:datatype="http://www.w3.org/2001/XMLSchema#date">2015-05-07</dcterms:created>
    <dcterms:partOf rdf:resource="http://vocab.deri.ie"/>
    <dcterms:type rdf:resource="http://purl.org/adms/assettype/Ontology"/>
    <dcterms:status rdf:resource="http://purl.org/adms/status/UnderDevelopment"/>
    <dc:creator rdf:resource="http://vocab.deri.ie/ac#wasder"/>
  </owl:Ontology>

  <adms:SemanticDistribution rdf:about="http://vocab.deri.ie/ac#ttl">
    <dcterms:FileFormat></dcterms:FileFormat>
    <adms:accessURL>http://vocab.deri.ie/ac.ttl</adms:accessURL>
    <adms:status rdf:resource="http://purl.org/adms/status/Completed"/>
  </adms:SemanticDistribution>

  <adms:SemanticDistribution rdf:about="http://vocab.deri.ie/ac#rdf">
    <dcterms:FileFormat></dcterms:FileFormat>
    <adms:accessURL>http://vocab.deri.ie/ac.rdf</adms:accessURL>
    <adms:status rdf:resource="http://purl.org/adms/status/Completed"/>
  </adms:SemanticDistribution>

  <foaf:Person rdf:about="http://vocab.deri.ie/ac#wasder">
    <foaf:name>Wassim Derguech</foaf:name>
    <foaf:homepage></foaf:homepage>
  </foaf:Person>

  <rdfs:Class rdf:about="http://vocab.deri.ie/ac#ActionCategory">
    <rdf:type rdf:resource="http://www.w3.org/2002/07/owl#Class"/>
    <rdfs:label>ActionCategory</rdfs:label>
    <rdfs:comment>This concept defines an action category.</rdfs:comment>
  </rdfs:Class>

  <rdf:Property rdf:about="http://vocab.deri.ie/ac#hasLevel">
    <rdf:type rdf:resource="http://www.w3.org/2002/07/owl#DatatypeProperty"/>
    <rdfs:label>level</rdfs:label>
    <rdfs:comment>This property allows to assign the level of an action category within a hierarchy of action categories.</rdfs:comment>
    <rdfs:domain rdf:resource="http://vocab.deri.ie/ac#ActionCategory"/>
    <rdfs:range rdf:resource="http://www.w3.org/2001/XMLSchema#integer"/>
  </rdf:Property>

  <rdf:Property rdf:about="http://vocab.deri.ie/ac#hasOptionalPart">
    <rdfs:label>hasOptionalPart</rdfs:label>
    <rdfs:comment>This property is used to create meronymy relation between actions. It is optional this means that an action can still be performed if its optional parts are not performed or absent</rdfs:comment>
    <rdfs:domain rdf:resource="http://vocab.deri.ie/ac#ActionCategory"/>
    <rdfs:range rdf:resource="http://vocab.deri.ie/ac#ActionCategory"/>
    <rdfs:subPropertyOf rdf:resource="http://vocab.deri.ie/ac#hasPart"/>
  </rdf:Property>

  <rdf:Property rdf:about="http://vocab.deri.ie/ac#hasPart">
    <rdfs:label>hasPart</rdfs:label>
    <rdfs:comment>This property is used to create meronymy relations between actions. An action category is performed only if all its parts are performed.</rdfs:comment>
    <rdfs:domain rdf:resource="http://vocab.deri.ie/ac#ActionCategory"/>
    <rdfs:range rdf:resource="http://vocab.deri.ie/ac#ActionCategory"/>
  </rdf:Property>

</rdf:RDF>